good progress using lref

state/TargetLangIFC.fst
@@ -10,40 +10,32 @@ open IFC.Heap.ST
 (** target_lang is a shallow embedding of STLC **)
 class target_lang (t:Type) = {
   deep_contains : lheap -> t -> Type0;
-  deeply_labeled : t -> lheap -> label -> Type0; (** deep check of the lebel of a value **)
+  deeply_labeled_with_low : t -> lheap -> Type0; (** deep check that the object points to low things **)
+
   deep_recall : (r:t) -> ST unit 
               (requires (fun h -> True))
-              (ensures  (fun h0 _ h1 -> h0 == h1 /\ h1 `deep_contains` r));
-  deep_declassify : (r:t) -> l:label -> ST unit 
-              (requires (fun h0 -> exists l0. deeply_labeled r h0 l0 /\ l0 `lattice_gte` l)) (* TODO: this does not work at all with loops *)
-              (ensures  (fun h0 _ h1 -> 
-                modifies_none h0 h1 /\
-                equal_dom h0 h1 /\
-                deeply_labeled r h1 l));
+              (ensures  (fun h0 _ h1 -> h0 == h1 /\ h1 `deep_contains` r /\ deeply_labeled_with_low r h1));  
 }
-
+  
 instance target_lang_unit : target_lang unit = {
   deep_contains = (fun _ _ -> True);
-  deeply_labeled = (fun _ _ _ -> True);
   deep_recall = (fun _ -> ());
-  deep_declassify = (fun _ _ -> ())
+
+  deeply_labeled_with_low = (fun _ _ -> True);
 }
 
 instance target_lang_int : target_lang int = {
   deep_contains = (fun _ _ -> True);
-  deeply_labeled = (fun _ _ _ -> True);
   deep_recall = (fun _ -> ());
-  deep_declassify = (fun _ _ -> ())
+
+  deeply_labeled_with_low = (fun _ _ -> True);
 }
 
 instance target_lang_pair (t1:Type) (t2:Type) {| c1:target_lang t1 |} {| c2:target_lang t2 |} : target_lang (t1 * t2) = {
   deep_contains = (fun h (x1, x2) -> h `deep_contains` x1 /\ h `deep_contains` x2);
-  deeply_labeled = (fun (x1, x2) h l -> c1.deeply_labeled x1 h l /\ c2.deeply_labeled x2 h l);
   deep_recall = (fun (x1, x2) -> c1.deep_recall x1; c2.deep_recall x2);
-  deep_declassify = (fun (x1, x2) l -> 
-    c1.deep_declassify x1 l; 
-    admit ();
-    c2.deep_declassify x2 l)
+
+  deeply_labeled_with_low = (fun (x1, x2) h -> c1.deeply_labeled_with_low x1 h /\ c2.deeply_labeled_with_low x2 h);
 }
 
 instance target_lang_sum (t1:Type) (t2:Type) {| c1:target_lang t1 |} {| c2:target_lang t2 |} : target_lang (either t1 t2) = {
@@ -51,60 +43,50 @@ instance target_lang_sum (t1:Type) (t2:Type) {| c1:target_lang t1 |} {| c2:targe
     match x with
     | Inl x1 -> h `deep_contains` x1
     | Inr x2 -> h `deep_contains` x2);
-  deeply_labeled = (fun x h l ->
-    match x with
-    | Inl x1 -> c1.deeply_labeled x1 h l
-    | Inr x2 -> c2.deeply_labeled x2 h l);
   deep_recall = (fun x ->
     match x with
     | Inl x1 -> c1.deep_recall x1
     | Inr x2 -> c2.deep_recall x2);
-  deep_declassify = (fun x l ->
+
+  deeply_labeled_with_low = (fun x h ->
     match x with
-    | Inl x1 -> c1.deep_declassify x1 l
-    | Inr x2 -> c2.deep_declassify x2 l)
+    | Inl x1 -> c1.deeply_labeled_with_low x1 h
+    | Inr x2 -> c2.deeply_labeled_with_low x2 h);
 }
 
-instance target_lang_ref (t:Type) {| c:target_lang t |} : target_lang (ref t) = {
-  deep_contains = (fun h (x:ref t) -> h `contains` x /\ h `deep_contains` (sel h x));
-  deeply_labeled = (fun (x:ref t) h l -> label_of x h == l /\ c.deeply_labeled (sel h x) h l);  
-  deep_recall = (fun (x:ref t) -> recall x; c.deep_recall !x);
-  deep_declassify = (fun (x:ref t) l -> 
-    declassify x l; 
-    admit ();
-    c.deep_declassify !x l
-  )
+instance target_lang_ref (t:Type) {| c:target_lang t |} : target_lang (lref t) = {
+  deep_contains = (fun h (x:lref t) -> h `contains` x /\ h `deep_contains` (sel h x));
+
+  deeply_labeled_with_low = (fun (x:lref t) h -> label_of x h == Low /\ c.deeply_labeled_with_low (sel h x) h);  
+  deep_recall = (fun (x:lref t) -> 
+    recall x; 
+    gst_recall (is_low_pred x);
+    c.deep_recall !x);
 }
 
-let modifies_only_label (l:label) (h0:lheap) (h1:lheap) : Type0 =
-  (forall (a:Type) (r:ref a). h0 `contains` r /\ label_of r h0 =!= l ==>
-          sel h0 r == sel h1 r)
+open FStar.Preorder
 
 let objects_deeply_labeled (h:lheap) : Type0 =
-  forall a (c:target_lang (ref a)) (r:ref a). h `contains` r ==> 
-    h `c.deep_contains` r /\ c.deeply_labeled r h (label_of r h)
+  forall a (c:target_lang (ref a)) (r:ref a). h `contains` r /\ label_of r h == Low ==> (* These are properties that can be recalled *)
+    h `c.deep_contains` r /\ c.deeply_labeled_with_low r h 
 
 unfold let pre_tgt_arrow
   (#t1:Type) (x:t1) {| tgtx:target_lang t1 |}
   (h0:lheap) =
-  objects_deeply_labeled h0 /\                                            (* all objects are deeply labeled *)
-  h0 `deep_contains` x /\                                                 (* required to instantiate the properties of modifies *)
-  deeply_labeled x h0 Tourist                                             (* x is a Tourist *)
+  objects_deeply_labeled h0 /\                                           (* all objects are deeply labeled *)
+  h0 `deep_contains` x /\                                                (* required to instantiate the properties of modifies *)
+  deeply_labeled_with_low x h0                                           (* x is Low *)
 
 let post_tgt_arrow
   (#t1:Type) (x:t1) {| tgtx:target_lang t1 |}
   (#t2:t1 -> Type) {| tgtr : (x:t1 -> target_lang (t2 x)) |}
   (h0:lheap) (r:t2 x) (h1:lheap) =
-  modifies_only_label Tourist h0 h1 /\                                  (* allow region rs to be modified *)
+  modifies_only_label Low h0 h1 /\                                       (* allow region rs to be modified *)
 
   objects_deeply_labeled h1 /\
 
   (h1 `(tgtr x).deep_contains` r) /\
-  ((tgtr x).deeply_labeled r h1 Tourist)                                  (* x is deeply labeled with Tourist *)
-(* TODO: what prevents the computation to allocate things in rp?
-    If necessary, we can dissable it by adding the following postcondition:
-      forall rrp. disjoint rrp rrs ==> equal_heap_dom rrp h0 h1 -- disables allocation in other regions
- *)
+  ((tgtr x).deeply_labeled_with_low r h1)                                (* r is deeply labeled with Low *)
 
 let mk_tgt_arrow 
   (t1:Type)
@@ -122,22 +104,273 @@ instance target_lang_arrow
   {| (x:t1 -> target_lang (t2 x)) |}
   : target_lang (mk_tgt_arrow t1 t2) = {
     deep_contains = (fun _ _ -> True);
-    deeply_labeled = (fun _ _ _ -> True);
     deep_recall = (fun _ -> ());
-    deep_declassify = (fun _ _ -> ())
+
+    deeply_labeled_with_low = (fun _ _ -> True);
   }
 
 let prog () =
   let r : ref int = alloc 0 in
   let h0 = get () in
-  assert (label_of r h0 == NoVisa);
-  declassify r Tourist;
-  assert (label_of r h0 == NoVisa);
+  assert (label_of r h0 == High);
+  declassify r Low;
+  assert (label_of r h0 == High);
   let h1 = get () in
-  assert (label_of r h1 == Tourist);
+  assert (label_of r h1 == Low);
   let r1 : ref int = alloc 0 in
-  declassify r1 Diplomatic;
+  declassify r1 Medium;
   ()
 
-(* TODO: during back-tarnslation, one needs to know that everything in env is deeply labeled with Tourist.
+(* TODO: during back-tarnslation, one needs to know that everything in env is deeply labeled with Low.
     previously, similar information (e.g., region) was on the reference *)
+
+open STLC
+
+(** *** Elaboration of types to F* *)
+let rec _elab_typ (t:typ) : tt:Type & target_lang tt =
+  match t with
+  | TArr t1 t2 -> begin
+    let tt1 = _elab_typ t1 in
+    let tt2 (x:dfst tt1) = _elab_typ t2 in
+    (| mk_tgt_arrow      (dfst tt1) #(dsnd tt1) (fun x -> dfst (tt2 x)) #(fun x -> dsnd (tt2 x)),
+       target_lang_arrow (dfst tt1) #(dsnd tt1) (fun x -> dfst (tt2 x)) #(fun x -> dsnd (tt2 x))
+    |)
+  end 
+  | TUnit -> (| unit, target_lang_unit |)
+  | TNat -> (| int, target_lang_int |)
+  | TSum t1 t2 ->
+    let (| tt1, c_tt1 |) = _elab_typ t1 in
+    let (| tt2, c_tt2 |) = _elab_typ t2 in
+    (| either tt1 tt2, target_lang_sum tt1 tt2 #c_tt1 #c_tt2 |)
+  | TPair t1 t2 ->
+    let (| tt1, c_tt1 |) = _elab_typ t1 in
+    let (| tt2, c_tt2 |) = _elab_typ t2 in
+    (| (tt1 * tt2), target_lang_pair tt1 tt2 #c_tt1 #c_tt2 |)
+  | TRef t ->
+    let (| tt, c_tt |) = _elab_typ t in
+    (| lref tt, target_lang_ref tt #c_tt |)
+
+let elab_typ (t:typ) : Type =
+  dfst (_elab_typ t)
+
+let elab_typ_tgt (t:typ) : target_lang (elab_typ t)=
+  dsnd (_elab_typ t)
+
+
+
+(** ** Examples **) 
+let write' (#t:Type) {| c:target_lang t |} (r:lref t) (v:t) 
+: ST unit
+  (requires (fun h0 -> 
+    h0 `deep_contains` r /\ h0 `c.deep_contains` v /\
+    label_of r h0 == Low /\ c.deeply_labeled_with_low v h0 /\
+    objects_deeply_labeled h0))
+  (ensures (fun h0 () h1 ->
+    write_post r v h0 () h1 /\
+    deeply_labeled_with_low r h1 /\
+    objects_deeply_labeled h1 /\
+    modifies_only_label Low h0 h1))
+= r := v;
+  let h1 = get () in
+  assume (deeply_labeled_with_low r h1);
+  assume (objects_deeply_labeled h1);
+  admit ();
+  ()
+
+
+val alloc' (#a:Type) {| c:target_lang a |} (init:a)
+: ST (lref a)
+  (requires (fun h0 ->
+    objects_deeply_labeled h0 /\
+    c.deeply_labeled_with_low init h0))
+  (ensures (fun h0 r h1 -> 
+    alloc_post init h0 r h1 /\
+    deeply_labeled_with_low r h1 /\ 
+    objects_deeply_labeled h1))
+let alloc' #_ #c v = 
+  let r = alloc v in
+  let r' = declassify_low r in
+  let h1 = get () in
+  assume (deeply_labeled_with_low r' h1);
+  assume (objects_deeply_labeled h1);
+  admit ();
+  r'
+
+val ctx_update_ref_test : 
+  elab_typ (TArr (TRef TNat) TUnit)
+let ctx_update_ref_test (y:lref int) =
+  write' y (!y + 5);
+  ()
+
+val ctx_update_multiple_refs_test : 
+  elab_typ (TArr (TRef (TRef TNat)) (TArr (TRef TNat) TUnit))
+let ctx_update_multiple_refs_test (x:lref (lref int)) (y:lref int) =
+  deep_recall x; (* Fstar forgets that x is contained and low **)
+  let ix : lref int = !x in
+  write' ix (!ix + 1);
+  deep_recall x; (* TODO: why is this one needed? *)
+  write' x y;
+  write' y (!y + 5);
+  ()
+
+val ctx_HO_test1 : 
+  elab_typ (TArr (TRef (TPair (TRef TNat) (TRef TNat))) (TArr TUnit TUnit))
+let ctx_HO_test1 (xs:lref ((lref int) * lref int)) =
+  let (x', x'') = !xs in
+  write' xs (x', x');  // xs := (x', x');
+  (fun () ->
+    deep_recall xs;
+    deep_recall x';
+    deep_recall x'';
+    write' xs (x', x'')
+  )
+  
+val ctx_identity :
+  elab_typ (TArr (TRef TNat) (TRef TNat))
+let ctx_identity x = x
+
+val ctx_HO_test2 :
+  elab_typ (TArr (TArr TUnit (TRef TNat)) TUnit)
+let ctx_HO_test2 f =
+  let h0 = get () in
+  let x:ref int = f () in
+  let h1 = get () in
+  // assert (lheap_rel h0 h1);
+  // assert (modifies_only_label Low h0 h1);
+  write' x (!x + 1);
+  let h2 = get () in
+  // assert (modifies_only_label Low h1 h2);
+  // assert (objects_deeply_labeled h2);
+  // assert (modifies_only_label Low h0 h2);
+  ()
+
+val ctx_swap_ref_test :
+  elab_typ (TArr (TRef (TRef TNat)) (TArr (TRef (TRef TNat)) TUnit))
+let ctx_swap_ref_test (x y: ref (ref int)) =
+  deep_recall x;
+  let h0 = get () in
+  assume (label_of x h0 == Low);
+  let z = !x in
+  let t = !y in
+  write' x t;
+  write' y z;
+  ()
+
+val ctx_dynamic_alloc_test :
+   elab_typ (TArr TUnit (TRef TNat))
+let ctx_dynamic_alloc_test () = 
+  let v = alloc' 0 in 
+  v
+
+val ctx_HO_test3 :
+  elab_typ (TArr (TArr TUnit (TRef TNat)) TUnit)
+let ctx_HO_test3 f =
+  let x:ref int = f () in
+  let y:ref int = alloc' (!x + 1) in
+  ()
+
+val ctx_returns_callback_test :
+  elab_typ (TArr TUnit (TArr TUnit TUnit))
+let ctx_returns_callback_test () =
+  let x: ref int = alloc' 13 in
+  let cb : elab_typ (TArr TUnit TUnit) = (fun() ->
+    recall x;
+    let h0 = get () in
+    assume (label_of x h0 == Low);
+    write' x (!x % 5)
+  ) in
+  cb
+
+val ctx_HO_test4 :
+  elab_typ (TArr (TArr TUnit (TRef TNat)) TUnit)
+let ctx_HO_test4 f =
+  let x:ref int = f () in
+  let y:ref (ref int) = alloc' x in
+  ()
+
+val progr_sep_test: 
+  #rp: ref int -> 
+  #rs: ref (ref int) ->
+  ctx:(elab_typ (TArr TUnit TUnit)) ->
+  ST unit
+    (requires (fun h0 -> 
+      label_of rp h0 == High /\
+      objects_deeply_labeled h0))
+    (ensures (fun h0 _ h1 ->
+      sel h0 rp == sel h1 rp)) // the content of rp should stay the same before/ after calling the context
+         
+let progr_sep_test #rp f = (** If this test fails, it means that the spec of f does not give [automatically] separation  **)
+  let h0 = get () in
+  assert (label_of rp h0 == High);
+  f ();
+  let h1 = get () in
+  // assert (label_of rp h1 == High);
+  assert (modifies_only_label Low h0 h1);
+  admit (); (** TODO: Figure out how to make this automatic *)
+  assert (sel h0 rp == sel h1 rp);
+  ()
+
+val progr_secret_unchanged_test: 
+  #rp: rref int -> 
+  #rs: rref (rref int) ->
+  #rrs:erid ->
+  #rrp:erid ->
+  ctx:(elab_typ (TArr TUnit TUnit) rrs) ->
+  ST unit 
+    (requires (fun h0 -> 
+      self_contained_region_inv rrs h0 /\
+      sep rp rrp rs rrs h0 /\
+      is_eternal_region rrs /\
+      is_eternal_region rrp))
+    (ensures (fun h0 _ h1 -> sep rp rrp rs rrs h1 /\
+                             sel h0 rp == sel h1 rp))
+         
+let progr_secret_unchanged_test #_ #rs #rrs #rrp ctx = 
+  let secret: rref int = ralloc' rrp 0 in
+  ctx ();
+  let v = !secret in
+  assert (v == 0);
+  deep_recall rs;
+  ()
+
+val progr_passing_callback_test: 
+  #rp: rref int -> 
+  #rs: rref (rref int) ->
+  #rrs:erid ->
+  #rrp:erid ->
+  ctx:(elab_typ (TArr (TArr TUnit TUnit) TUnit) rrs) ->
+  ST unit 
+    (requires (fun h0 -> 
+      self_contained_region_inv rrs h0 /\
+      sep rp rrp rs rrs h0 /\
+      is_eternal_region rrs))
+    (ensures (fun h0 _ h1 -> sep rp rrp rs rrs h1 /\
+                             sel h0 rp == sel h1 rp)) // the content of rp should stay the same before/ after calling the context
+
+// TODO: the callback of the program should be able to modify rp
+let progr_passing_callback_test #_ #rs #rrs #rrp f =
+  let secret: rref int = ralloc' rrs 0 in
+  let cb: elab_typ (TArr TUnit TUnit) rrs = (fun () -> write' secret (!secret + 1)) in
+  f cb;
+  deep_recall rs;
+  ()
+
+val progr_getting_callback_test: 
+  #rp: rref int -> 
+  #rs: rref (rref int) ->
+  #rrs:erid ->
+  #rrp:erid ->
+  ctx:(elab_typ (TArr TUnit (TArr TUnit TUnit)) rrs) ->
+  ST unit 
+    (requires (fun h0 -> 
+      self_contained_region_inv rrs h0 /\
+      sep rp rrp rs rrs h0 /\
+      is_eternal_region rrs))
+    (ensures (fun h0 _ h1 -> sep rp rrp rs rrs h1 /\
+                             sel h0 rp == sel h1 rp))
+
+let progr_getting_callback_test #_ #rs #rrs #rrp f =
+  let cb = f () in
+  cb ();
+  deep_recall rs;
+  ()
